this might actually get me through

theories/Logic/neg_inverse_omega.v
@@ -30,9 +30,14 @@ Qed.
 Fixpoint neg_w_rule_sub_ptree_fit
   (P Q : ptree) (E F : formula) (n d' : nat) (beta : ord) (H : P_proves Q (lor F (univ n E)) d' beta) (S : subst_ind) : ptree :=
   match P, S with
-| deg_up d P', _ => deg_up d (neg_w_rule_sub_ptree_fit P' Q E F n d' beta H S)
-
-| ord_up alpha P', _ => ord_up alpha (neg_w_rule_sub_ptree_fit P' Q E F n d' beta H S)
+| deg_up d P', _ => match lt_nat (ptree_deg (neg_w_rule_sub_ptree_fit P' Q E F n d' beta H S)) d with
+    | true => deg_up d (neg_w_rule_sub_ptree_fit P' Q E F n d' beta H S)
+    | false => (neg_w_rule_sub_ptree_fit P' Q E F n d' beta H S)
+    end
+| ord_up alpha P', _ => match ord_ltb (ptree_ord (neg_w_rule_sub_ptree_fit P' Q E F n d' beta H S)) alpha with
+    | true => ord_up alpha (neg_w_rule_sub_ptree_fit P' Q E F n d' beta H S)
+    | false => (neg_w_rule_sub_ptree_fit P' Q E F n d' beta H S)
+    end
 
 | node A, _ => P
 
@@ -40,7 +45,8 @@ Fixpoint neg_w_rule_sub_ptree_fit
     exchange_ab
       (neg_w_rule_sub_formula A E F n S_A)
       (neg_w_rule_sub_formula B E F n S_B)
-      d alpha
+      (ptree_deg (neg_w_rule_sub_ptree_fit P' Q E F n d' beta H (lor_ind S_A S_B)))
+      (ptree_ord (neg_w_rule_sub_ptree_fit P' Q E F n d' beta H (lor_ind S_A S_B)))
       (neg_w_rule_sub_ptree_fit P' Q E F n d' beta H (lor_ind S_A S_B))
 
 | exchange_cab C A B d alpha P', lor_ind (lor_ind S_C S_B) S_A =>
@@ -48,7 +54,8 @@ Fixpoint neg_w_rule_sub_ptree_fit
       (neg_w_rule_sub_formula C E F n S_C)
       (neg_w_rule_sub_formula A E F n S_A)
       (neg_w_rule_sub_formula B E F n S_B)
-      d alpha
+      (ptree_deg (neg_w_rule_sub_ptree_fit P' Q E F n d' beta H (lor_ind (lor_ind S_C S_A) S_B)))
+      (ptree_ord (neg_w_rule_sub_ptree_fit P' Q E F n d' beta H (lor_ind (lor_ind S_C S_A) S_B)))
       (neg_w_rule_sub_ptree_fit P' Q E F n d' beta H (lor_ind (lor_ind S_C S_A) S_B))
 
 | exchange_abd A B D d alpha P', lor_ind (lor_ind S_B S_A) S_D =>
@@ -56,7 +63,8 @@ Fixpoint neg_w_rule_sub_ptree_fit
       (neg_w_rule_sub_formula A E F n S_A)
       (neg_w_rule_sub_formula B E F n S_B)
       (neg_w_rule_sub_formula D E F n S_D)
-      d alpha
+      (ptree_deg (neg_w_rule_sub_ptree_fit P' Q E F n d' beta H (lor_ind (lor_ind S_A S_B) S_D)))
+      (ptree_ord (neg_w_rule_sub_ptree_fit P' Q E F n d' beta H (lor_ind (lor_ind S_A S_B) S_D)))
       (neg_w_rule_sub_ptree_fit P' Q E F n d' beta H (lor_ind (lor_ind S_A S_B) S_D))
 
 | exchange_cabd C A B D d alpha P', lor_ind (lor_ind (lor_ind S_C S_B) S_A) S_D =>
@@ -65,29 +73,31 @@ Fixpoint neg_w_rule_sub_ptree_fit
       (neg_w_rule_sub_formula A E F n S_A)
       (neg_w_rule_sub_formula B E F n S_B)
       (neg_w_rule_sub_formula D E F n S_D)
-      d alpha
-      (neg_w_rule_sub_ptree_fit
-        P' Q E F n d' beta H
-        (lor_ind (lor_ind (lor_ind S_C S_A) S_B) S_D))
+      (ptree_deg (neg_w_rule_sub_ptree_fit P' Q E F n d' beta H (lor_ind (lor_ind (lor_ind S_C S_A) S_B) S_D)))
+      (ptree_ord (neg_w_rule_sub_ptree_fit P' Q E F n d' beta H (lor_ind (lor_ind (lor_ind S_C S_A) S_B) S_D)))
+      (neg_w_rule_sub_ptree_fit P' Q E F n d' beta H (lor_ind (lor_ind (lor_ind S_C S_A) S_B) S_D))
 
 | contraction_a A d alpha P', _ =>
     contraction_a
       (neg_w_rule_sub_formula A E F n S)
-      d alpha
+      (ptree_deg (neg_w_rule_sub_ptree_fit P' Q E F n d' beta H (lor_ind S S)))
+      (ptree_ord (neg_w_rule_sub_ptree_fit P' Q E F n d' beta H (lor_ind S S)))
       (neg_w_rule_sub_ptree_fit P' Q E F n d' beta H (lor_ind S S))
 
 | contraction_ad A D d alpha P', lor_ind S_A S_D =>
     contraction_ad
       (neg_w_rule_sub_formula A E F n S_A)
       (neg_w_rule_sub_formula D E F n S_D)
-      d alpha
+      (ptree_deg (neg_w_rule_sub_ptree_fit P' Q E F n d' beta H (lor_ind (lor_ind S_A S_A) S_D)))
+      (ptree_ord (neg_w_rule_sub_ptree_fit P' Q E F n d' beta H (lor_ind (lor_ind S_A S_A) S_D)))
       (neg_w_rule_sub_ptree_fit P' Q E F n d' beta H (lor_ind (lor_ind S_A S_A) S_D))
 
 | weakening_ad A D d alpha P', lor_ind S_A S_D =>
     weakening_ad
       (neg_w_rule_sub_formula A E F n S_A)
       (neg_w_rule_sub_formula D E F n S_D)
-      d alpha
+      (ptree_deg (neg_w_rule_sub_ptree_fit P' Q E F n d' beta H S_D))
+      (ptree_ord (neg_w_rule_sub_ptree_fit P' Q E F n d' beta H S_D))
       (neg_w_rule_sub_ptree_fit P' Q E F n d' beta H S_D)
 
 | demorgan_ab A B d1 d2 alpha1 alpha2 P1 P2, _ => P
@@ -96,7 +106,10 @@ Fixpoint neg_w_rule_sub_ptree_fit
     demorgan_abd
       A B
       (neg_w_rule_sub_formula D E F n S_D)
-      d1 d2 alpha1 alpha2
+      (ptree_deg (neg_w_rule_sub_ptree_fit P1 Q E F n d' beta H (lor_ind (0) S_D)))
+      (ptree_deg (neg_w_rule_sub_ptree_fit P2 Q E F n d' beta H (lor_ind (0) S_D)))
+      (ptree_ord (neg_w_rule_sub_ptree_fit P1 Q E F n d' beta H (lor_ind (0) S_D)))
+      (ptree_ord (neg_w_rule_sub_ptree_fit P2 Q E F n d' beta H (lor_ind (0) S_D)))
       (neg_w_rule_sub_ptree_fit P1 Q E F n d' beta H (lor_ind (0) S_D))
       (neg_w_rule_sub_ptree_fit P2 Q E F n d' beta H (lor_ind (0) S_D))
 
@@ -106,22 +119,23 @@ Fixpoint neg_w_rule_sub_ptree_fit
     negation_ad
       A
       (neg_w_rule_sub_formula D E F n S_D)
-      d alpha
+      (ptree_deg (neg_w_rule_sub_ptree_fit P' Q E F n d' beta H (lor_ind (non_target A) S_D)))
+      (ptree_ord (neg_w_rule_sub_ptree_fit P' Q E F n d' beta H (lor_ind (non_target A) S_D)))
       (neg_w_rule_sub_ptree_fit P' Q E F n d' beta H (lor_ind (non_target A) S_D))
 
 | quantification_a A k t d alpha P', _ =>
     (match eq_f A E, eq_nat k n, S with
-    | true, true, (1) => (cut_ca F (substitution E n t) d' d beta alpha (projT1(w_rule_invertible_cut_cad Q E F n d' beta t H)) P')
+    | true, true, (1) => (cut_ca F (substitution E n (projT1 t)) (ptree_deg (w_rule_sub_ptree Q E n t (lor_ind (non_target F) (1)))) d beta alpha (w_rule_sub_ptree Q E n t (lor_ind (non_target F) (1))) P')
     | _, _, _ => P
     end)
 
 | quantification_ad A D k t d alpha P', lor_ind S_A S_D =>
     (match eq_f A E, eq_nat k n, S_A with
-    | true, true, (1) => (cut_cad F (substitution E n t) (neg_w_rule_sub_formula D E F n S_D) d' d beta alpha (projT1(w_rule_invertible_cut_cad Q E F n (eval t - 1) d' beta H)) P')
+    | true, true, (1) => (cut_cad F (substitution E n (projT1 t)) (neg_w_rule_sub_formula D E F n S_D) d' d beta alpha (projT1(w_rule_invertible_cut_cad Q E F n d' beta t H)) P')
     | _, _, _ => quantification_ad
-                    A
-                    (neg_w_rule_sub_formula D E F n S_D)
-                    k t d alpha
+                    A (neg_w_rule_sub_formula D E F n S_D) k t
+                    (ptree_deg (neg_w_rule_sub_ptree_fit P' Q E F n d' beta H (lor_ind (0) S_D)))
+                    (ptree_ord (neg_w_rule_sub_ptree_fit P' Q E F n d' beta H (lor_ind (0) S_D)))
                     (neg_w_rule_sub_ptree_fit P' Q E F n d' beta H (lor_ind (0) S_D))
     end)
 
@@ -129,33 +143,33 @@ Fixpoint neg_w_rule_sub_ptree_fit
 
 | w_rule_ad A D k d alpha g, lor_ind S_A S_D =>
     w_rule_ad
-          A
-          (neg_w_rule_sub_formula D E F n S_D)
-          k d alpha
-          (fun (p : nat) =>
-            neg_w_rule_sub_ptree_fit (g p) Q E F n d' beta H (lor_ind (non_target A) S_D))
+          A (neg_w_rule_sub_formula D E F n S_D) k
+          (ptree_deg (neg_w_rule_sub_ptree_fit (g czero) Q E F n d' beta H (lor_ind (non_target A) S_D)))
+          (ord_2_exp alpha)
+          (fun (c : c_term) =>
+            neg_w_rule_sub_ptree_fit (g c) Q E F n d' beta H (lor_ind (non_target A) S_D))
 
 | cut_ca C A d1 d2 alpha1 alpha2 P1 P2, _ =>
     cut_ca
-      (neg_w_rule_sub_formula C E F n S)
-      A d1 d2 alpha1 alpha2
-      (neg_w_rule_sub_ptree_fit P1 Q E F n d' beta H (lor_ind S (non_target A)))
-      P2
+      (neg_w_rule_sub_formula C E F n S) A
+      (ptree_deg (neg_w_rule_sub_ptree_fit P1 Q E F n d' beta H (lor_ind S (non_target A)))) d2
+      (ptree_ord (neg_w_rule_sub_ptree_fit P1 Q E F n d' beta H (lor_ind S (non_target A)))) alpha2
+      (neg_w_rule_sub_ptree_fit P1 Q E F n d' beta H (lor_ind S (non_target A)))  P2
 
 | cut_ad A D d1 d2 alpha1 alpha2 P1 P2, _ =>
     cut_ad
-      A
-      (neg_w_rule_sub_formula D E F n S)
-      d1 d2 alpha1 alpha2
-      P1
-      (neg_w_rule_sub_ptree_fit P2 Q E F n d' beta H (lor_ind (0) S))
+      A (neg_w_rule_sub_formula D E F n S)
+      d1 (ptree_deg (neg_w_rule_sub_ptree_fit P2 Q E F n d' beta H (lor_ind (0) S)))
+      alpha1 (ptree_ord (neg_w_rule_sub_ptree_fit P2 Q E F n d' beta H (lor_ind (0) S)))
+      P1   (neg_w_rule_sub_ptree_fit P2 Q E F n d' beta H (lor_ind (0) S))
 
 | cut_cad C A D d1 d2 alpha1 alpha2 P1 P2, lor_ind S_C S_D =>
     cut_cad
-      (neg_w_rule_sub_formula C E F n S_C)
-      A
-      (neg_w_rule_sub_formula D E F n S_D)
-      d1 d2 alpha1 alpha2
+      (neg_w_rule_sub_formula C E F n S_C) A (neg_w_rule_sub_formula D E F n S_D)
+      (ptree_deg (neg_w_rule_sub_ptree_fit P1 Q E F n d' beta H (lor_ind S_C (non_target A))))
+      (ptree_deg (neg_w_rule_sub_ptree_fit P2 Q E F n d' beta H (lor_ind (0) S_D)))
+      (ptree_ord (neg_w_rule_sub_ptree_fit P1 Q E F n d' beta H (lor_ind S_C (non_target A))))
+      (ptree_ord (neg_w_rule_sub_ptree_fit P2 Q E F n d' beta H (lor_ind (0) S_D)))
       (neg_w_rule_sub_ptree_fit P1 Q E F n d' beta H (lor_ind S_C (non_target A)))
       (neg_w_rule_sub_ptree_fit P2 Q E F n d' beta H (lor_ind (0) S_D))
 
@@ -207,11 +221,11 @@ induction P; try intros H S Hs.
 
 - simpl in Hs. simpl. rewrite Hs. simpl.
   rewrite (neg_w_rule_ptree_formula_true _ _ _ _ _ _ _ _ _ Hs).
-  destruct H as [H1 H2]. apply (IHP H2). auto.
+  destruct H as [H1 H2]. case (lt_nat (ptree_deg (neg_w_rule_sub_ptree P Q E F n d' beta HQ S)) n0); apply (IHP H2); auto.
 
 - simpl in Hs. simpl. rewrite Hs. simpl.
   rewrite (neg_w_rule_ptree_formula_true _ _ _ _ _ _ _ _ _ Hs).
-  destruct H as [[H1 H2] H3]. apply (IHP H2). auto.
+  destruct H as [[H1 H2] H3]. case (ord_ltb (ptree_ord (neg_w_rule_sub_ptree P Q E F n d' beta HQ S)) o); apply (IHP H2); auto.
 
 - simpl. inversion H.
   destruct (axiom_atomic _ H1); destruct H0; rewrite H0;
@@ -317,17 +331,17 @@ Qed.
 
 
 
-
+(*
 
 (* Second, we must prove that neg_w_rule_sub_ptree does not change the degree
 of an ptree. *)
 (* *)
 Lemma  neg_w_rule_ptree_deg : forall (P Q : ptree) (E F : formula) (n d' : nat) (beta : ord) (H : P_proves Q (lor F (univ n E)) d' beta),
   valid P ->
-  forall (S : subst_ind), (Nat.max (Nat.max d' (ptree_deg P)) ((num_conn E) + 1)) = ptree_deg (neg_w_rule_sub_ptree P Q E F n d' beta H S).
+    forall (S : subst_ind), (Nat.max (Nat.max d' (ptree_deg P)) ((num_conn E) + 1)) = ptree_deg (neg_w_rule_sub_ptree P Q E F n d' beta H S).
 Proof.
-intros P Q E F n d' beta HQ H. induction P; intros S.
-- simpl. case (subst_ind_fit (ptree_formula P) S); auto.
+intros P Q E F n d' beta HQ H. induction P; intros S I1 I2; simpl in I1,I2.
+- simpl. case (subst_ind_fit (ptree_formula P) S); simpl; auto. lia.
 - simpl. case (subst_ind_fit (ptree_formula P) S) eqn:Hfit; auto. simpl.
   rewrite (neg_w_rule_ptree_formula_true _ _ _ _ _ _ _ _ _ Hfit).
   apply IHP. inversion H. destruct X. auto.
@@ -367,88 +381,289 @@ intros P Q E F n d' beta HQ H. induction P; intros S.
   destruct S; auto. destruct (subst_ind_fit f S1 && subst_ind_fit f1 S2); auto.
 Admitted.
 
+*)
+
 
 (* Third, we must prove that neg_w_rule_sub_ptree does not change the ordinal
 of an ptree. *)
 (* *)
 Lemma neg_w_rule_ptree_ord : forall (P Q : ptree) (E F : formula) (n d' : nat) (beta : ord) (H : P_proves Q (lor F (univ n E)) d' beta),
   valid P ->
-  forall (S : subst_ind), ptree_ord (neg_w_rule_sub_ptree P Q E F n d' beta H S) = ptree_ord P.
+  forall (S : subst_ind), ord_ltb (ord_2_exp (ptree_ord P)) (ptree_ord (neg_w_rule_sub_ptree P Q E F n d' beta H S)) = false.
 Proof.
 intros P Q E F n d' beta HQ H. induction P; intros S.
-- simpl. case (subst_ind_fit (ptree_formula P) S) eqn:Hfit; auto. simpl.
-  rewrite (neg_w_rule_ptree_formula_true _ _ _ _ _ _ _ _ _ Hfit).
-  apply IHP. inversion H. auto.
-- simpl. case (subst_ind_fit (ptree_formula P) S); auto.
+- simpl. case (subst_ind_fit (ptree_formula P) S) eqn:Hfit; auto. 
+  + case (lt_nat (ptree_deg (neg_w_rule_sub_ptree_fit P Q E F n d' beta HQ S)) n0) eqn:X;
+    destruct H; simpl; rewrite neg_w_rule_ptree_formula_true; auto. 
+  + destruct H. destruct (ord_2_exp_fp _ (ptree_ord_nf _ v)).
+    * apply ltb_asymm. apply ord_lt_ltb. auto.
+    * simpl. rewrite H. auto. 
+- simpl. case (subst_ind_fit (ptree_formula P) S) eqn:Y; auto.
+  + case (ord_ltb (ptree_ord (neg_w_rule_sub_ptree_fit P Q E F n d' beta HQ S)) o) eqn:X; destruct H as [[H1 H2] H3]; simpl.
+    * simpl. destruct (ord_2_exp_fp _ H3).
+      --  apply ltb_asymm. apply ord_lt_ltb. auto.
+      --  simpl. rewrite H. auto.
+    * rewrite neg_w_rule_ptree_formula_true; auto. apply ltb_asymm. case (ord_eqb (ord_2_exp (ptree_ord P)) (ptree_ord (neg_w_rule_sub_ptree P Q E F n d' beta HQ S))) eqn:Z.
+      --  apply ord_eqb_eq in Z. destruct Z. apply ord_lt_ltb. apply ord_2_exp_monot; auto. apply ptree_ord_nf; auto.
+      --  refine (ord_ltb_trans _ _ _ _ (ord_lt_ltb _ _ (ord_2_exp_monot _ _ _ _ H1))); auto.
+          pose proof (IHP H2 S). destruct (ord_semiconnex_bool (ptree_ord (neg_w_rule_sub_ptree P Q E F n d' beta HQ S)) (ord_2_exp (ptree_ord P))) as [O | [O| O]]; auto.
+          rewrite O in H. inversion H. apply ord_eqb_eq in O. destruct O. rewrite ord_eqb_refl in Z. inversion Z. apply ptree_ord_nf; auto.
+  + simpl. destruct H. destruct (ord_2_exp_fp _ n0).
+    * apply ltb_asymm. apply ord_lt_ltb. auto.
+    * simpl. rewrite H. auto. 
 - simpl. case (subst_ind_fit f S); auto.
-- simpl.
-  destruct S; auto. case (subst_ind_fit f0 S1 && subst_ind_fit f S2); auto.
-- simpl. destruct S; auto. destruct S1; auto.
-  case (subst_ind_fit f S1_1 && subst_ind_fit f1 S1_2 && subst_ind_fit f0 S2);
-  auto.
-- simpl. destruct S; auto. destruct S1; auto.
-  case (subst_ind_fit f0 S1_1 && subst_ind_fit f S1_2 && subst_ind_fit f1 S2);
-  auto.
-- simpl. destruct S; auto. destruct S1; auto. destruct S1_1; auto.
-  case (subst_ind_fit f S1_1_1 && subst_ind_fit f1 S1_1_2 &&
-        subst_ind_fit f0 S1_2 && subst_ind_fit f2 S2); auto.
-- simpl. destruct (subst_ind_fit f S); auto.
-- simpl.
-  destruct S; auto. destruct (subst_ind_fit f S1 && subst_ind_fit f0 S2); auto.
-- simpl.
-  destruct S; auto. destruct (subst_ind_fit f S1 && subst_ind_fit f0 S2); auto.
 - simpl. destruct S; auto.
-- simpl. destruct S; auto. destruct S1; destruct (subst_ind_fit f1 S2); auto.
+  + simpl. destruct H as [[[X1 X2] X3] X4]. rewrite X4. destruct (ord_2_exp_fp _ (ptree_ord_nf _ X2)).
+    * apply ltb_asymm. apply ord_lt_ltb. auto.
+    * simpl. rewrite H. auto. 
+  + simpl. destruct H as [[[X1 X2] X3] X4]. rewrite X4. destruct (ord_2_exp_fp _ (ptree_ord_nf _ X2)).
+    * apply ltb_asymm. apply ord_lt_ltb. auto.
+    * simpl. rewrite H. auto. 
+  + case (subst_ind_fit f0 S1 && subst_ind_fit f S2) eqn:X; auto.
+    * simpl. destruct H as [[[X1 X2] X3] X4]. rewrite X4. rewrite neg_w_rule_ptree_formula_true. apply IHP; auto.
+      rewrite X1. simpl. apply and_bool_symm. auto.
+    * simpl. destruct H as [[[X1 X2] X3] X4]. rewrite X4. destruct (ord_2_exp_fp _ (ptree_ord_nf _ X2)).
+      --  apply ltb_asymm. apply ord_lt_ltb. auto.
+      --  simpl. rewrite H. auto.  
 - simpl. destruct S; auto.
+  + simpl. destruct H as [[[X1 X2] X3] X4]. rewrite X4. destruct (ord_2_exp_fp _ (ptree_ord_nf _ X2)).
+    * apply ltb_asymm. apply ord_lt_ltb. auto.
+    * simpl. rewrite H. auto. 
+  + simpl. destruct H as [[[X1 X2] X3] X4]. rewrite X4. destruct (ord_2_exp_fp _ (ptree_ord_nf _ X2)).
+    * apply ltb_asymm. apply ord_lt_ltb. auto.
+    * simpl. rewrite H. auto. 
+  + destruct S1; auto.
+    * simpl. destruct H as [[[X1 X2] X3] X4]. rewrite X4. destruct (ord_2_exp_fp _ (ptree_ord_nf _ X2)).
+      --  apply ltb_asymm. apply ord_lt_ltb. auto.
+      --  simpl. rewrite H. auto.
+    * simpl. destruct H as [[[X1 X2] X3] X4]. rewrite X4. destruct (ord_2_exp_fp _ (ptree_ord_nf _ X2)).
+      --  apply ltb_asymm. apply ord_lt_ltb. auto.
+      --  simpl. rewrite H. auto.
+    * case (subst_ind_fit f S1_1 && subst_ind_fit f1 S1_2 && subst_ind_fit f0 S2) eqn:X; auto.
+      --  simpl. destruct H as [[[X1 X2] X3] X4]. rewrite X4. rewrite neg_w_rule_ptree_formula_true. apply IHP; auto.
+          rewrite X1. simpl. destruct (and_bool_prop _ _ X). destruct (and_bool_prop _ _ H). rewrite H0,H1,H2. auto.
+      --  simpl. destruct H as [[[X1 X2] X3] X4]. rewrite X4. destruct (ord_2_exp_fp _ (ptree_ord_nf _ X2)).
+          ++  apply ltb_asymm. apply ord_lt_ltb. auto.
+          ++  simpl. rewrite H. auto. 
 - simpl. destruct S; auto.
-  destruct S1; destruct (subst_ind_fit f0 S2) eqn:HS2; auto.
-- simpl. destruct S; auto. admit. admit.
-- simpl.
-  destruct S; auto; destruct S1; auto; destruct (subst_ind_fit f0 S2); auto. admit. admit.
+  + simpl. destruct H as [[[X1 X2] X3] X4]. rewrite X4. destruct (ord_2_exp_fp _ (ptree_ord_nf _ X2)).
+    * apply ltb_asymm. apply ord_lt_ltb. auto.
+    * simpl. rewrite H. auto. 
+  + simpl. destruct H as [[[X1 X2] X3] X4]. rewrite X4. destruct (ord_2_exp_fp _ (ptree_ord_nf _ X2)).
+    * apply ltb_asymm. apply ord_lt_ltb. auto.
+    * simpl. rewrite H. auto. 
+  + destruct S1; auto.
+    * simpl. destruct H as [[[X1 X2] X3] X4]. rewrite X4. destruct (ord_2_exp_fp _ (ptree_ord_nf _ X2)).
+      --  apply ltb_asymm. apply ord_lt_ltb. auto.
+      --  simpl. rewrite H. auto.
+    * simpl. destruct H as [[[X1 X2] X3] X4]. rewrite X4. destruct (ord_2_exp_fp _ (ptree_ord_nf _ X2)).
+      --  apply ltb_asymm. apply ord_lt_ltb. auto.
+      --  simpl. rewrite H. auto.
+    * case (subst_ind_fit f0 S1_1 && subst_ind_fit f S1_2 && subst_ind_fit f1 S2) eqn:X; auto.
+      --  simpl. destruct H as [[[X1 X2] X3] X4]. rewrite X4. rewrite neg_w_rule_ptree_formula_true. apply IHP; auto.
+          rewrite X1. simpl. destruct (and_bool_prop _ _ X). destruct (and_bool_prop _ _ H). rewrite H0,H1,H2. auto.
+      --  simpl. destruct H as [[[X1 X2] X3] X4]. rewrite X4. destruct (ord_2_exp_fp _ (ptree_ord_nf _ X2)).
+          ++  apply ltb_asymm. apply ord_lt_ltb. auto.
+          ++  simpl. rewrite H. auto. 
 - simpl. destruct S; auto.
-- simpl. destruct S; auto; destruct S1; auto; destruct (subst_ind_fit f0 S2) eqn:HS2; auto. 
-- simpl. destruct (subst_ind_fit f S); auto.
-- simpl. destruct (subst_ind_fit f0 S); auto.
-- simpl. destruct S; auto. destruct (subst_ind_fit f S1 && subst_ind_fit f1 S2); auto.
+  + simpl. destruct H as [[[X1 X2] X3] X4]. rewrite X4. destruct (ord_2_exp_fp _ (ptree_ord_nf _ X2)).
+    * apply ltb_asymm. apply ord_lt_ltb. auto.
+    * simpl. rewrite H. auto. 
+  + simpl. destruct H as [[[X1 X2] X3] X4]. rewrite X4. destruct (ord_2_exp_fp _ (ptree_ord_nf _ X2)).
+    * apply ltb_asymm. apply ord_lt_ltb. auto.
+    * simpl. rewrite H. auto. 
+  + destruct S1; auto.
+    * simpl. destruct H as [[[X1 X2] X3] X4]. rewrite X4. destruct (ord_2_exp_fp _ (ptree_ord_nf _ X2)).
+      --  apply ltb_asymm. apply ord_lt_ltb. auto.
+      --  simpl. rewrite H. auto.
+    * simpl. destruct H as [[[X1 X2] X3] X4]. rewrite X4. destruct (ord_2_exp_fp _ (ptree_ord_nf _ X2)).
+      --  apply ltb_asymm. apply ord_lt_ltb. auto.
+      --  simpl. rewrite H. auto.
+    * destruct S1_1.
+      --  simpl. destruct H as [[[X1 X2] X3] X4]. rewrite X4. destruct (ord_2_exp_fp _ (ptree_ord_nf _ X2)).
+          ++  apply ltb_asymm. apply ord_lt_ltb. auto.
+          ++  simpl. rewrite H. auto.
+      --  simpl. destruct H as [[[X1 X2] X3] X4]. rewrite X4. destruct (ord_2_exp_fp _ (ptree_ord_nf _ X2)).
+          ++  apply ltb_asymm. apply ord_lt_ltb. auto.
+          ++  simpl. rewrite H. auto.
+      --  case (subst_ind_fit f S1_1_1 && subst_ind_fit f1 S1_1_2 && subst_ind_fit f0 S1_2 && subst_ind_fit f2 S2) eqn:X; auto.
+          ++  simpl. destruct H as [[[X1 X2] X3] X4]. rewrite X4. rewrite neg_w_rule_ptree_formula_true. apply IHP; auto.
+              rewrite X1. simpl. destruct (and_bool_prop _ _ X). destruct (and_bool_prop _ _ H). destruct (and_bool_prop _ _ H1). rewrite H0,H2,H3,H4. auto.
+          ++  simpl. destruct H as [[[X1 X2] X3] X4]. rewrite X4. destruct (ord_2_exp_fp _ (ptree_ord_nf _ X2)).
+              **  apply ltb_asymm. apply ord_lt_ltb. auto.
+              **  simpl. rewrite H. auto.
+- simpl. destruct H as [[[X1 X2] X3] X4]. case (subst_ind_fit f S) eqn:X.
+  + simpl. rewrite neg_w_rule_ptree_formula_true.
+    * destruct X4. apply IHP. auto.
+    * rewrite X1. simpl. rewrite X. auto.
+  + simpl. rewrite X4. destruct (ord_2_exp_fp _ (ptree_ord_nf _ X2)).
+    * apply ltb_asymm. apply ord_lt_ltb. auto.
+    * simpl. rewrite H. auto.
+- simpl. destruct H as [[[X1 X2] X3] X4]. destruct S.
+  + simpl. rewrite X4. destruct (ord_2_exp_fp _ (ptree_ord_nf _ X2)).
+    * apply ltb_asymm. apply ord_lt_ltb. auto.
+    * simpl. rewrite H. auto.
+  + simpl. rewrite X4. destruct (ord_2_exp_fp _ (ptree_ord_nf _ X2)).
+    * apply ltb_asymm. apply ord_lt_ltb. auto.
+    * simpl. rewrite H. auto.
+  + case (subst_ind_fit f S1 && subst_ind_fit f0 S2) eqn:X.
+    * simpl. rewrite neg_w_rule_ptree_formula_true.
+      --  destruct X4. apply IHP. auto.
+      --  rewrite X1. simpl. destruct (and_bool_prop _ _ X). rewrite H,H0. auto.
+    * simpl. rewrite X4. destruct (ord_2_exp_fp _ (ptree_ord_nf _ X2)).
+      --  apply ltb_asymm. apply ord_lt_ltb. auto.
+      --  simpl. rewrite H. auto.
+- simpl. destruct S; auto.
+  + simpl. destruct H as [[[X1 X2] X3] X4]. rewrite X4. apply ltb_asymm. apply ord_lt_ltb. apply ord_succ_not_exp_fp. apply ord_succ_nf. apply (ptree_ord_nf _ X2).
+  + simpl. destruct H as [[[X1 X2] X3] X4]. rewrite X4. apply ltb_asymm. apply ord_lt_ltb. apply ord_succ_not_exp_fp. apply ord_succ_nf. apply (ptree_ord_nf _ X2).
+  + case (subst_ind_fit f S1 && subst_ind_fit f0 S2) eqn:X; auto.
+    * simpl. destruct H as [[[[X0 X1] X2] X3] X4]. rewrite X4. rewrite neg_w_rule_ptree_formula_true. destruct (ord_semiconnex_bool (ord_2_exp (ptree_ord P)) (ptree_ord (neg_w_rule_sub_ptree P Q E F n d' beta HQ S2))) as [O | [O | O]].
+      -- apply ltb_asymm. rewrite IHP in O. inversion O. auto.
+      -- destruct o.
+          ++ destruct X4. simpl in O. rewrite (ord_lt_one _ (ord_ltb_lt _ _ O)). auto.
+          ++ apply ltb_asymm. apply (ord_ltb_trans _ _ _ (ord_lt_ltb _ _ (ord_lt_succ _ _ (ord_ltb_lt _ _ O)))). apply ord_lt_ltb. apply ord_succ_lt_exp_succ. apply ptree_ord_nf; auto. destruct X4. apply zero_lt.
+      --  apply ord_eqb_eq in O. destruct O. case (ptree_ord P) eqn:Y; auto. apply ltb_asymm. apply ord_lt_ltb. apply ord_succ_lt_exp_succ. destruct Y. apply ptree_ord_nf; auto. apply zero_lt.
+      --  destruct (and_bool_prop _ _ X). rewrite X0. auto.
+    * simpl. destruct H as [[[X1 X2] X3] X4]. rewrite X4. apply ltb_asymm. apply ord_lt_ltb. apply ord_succ_not_exp_fp. apply ord_succ_nf. apply (ptree_ord_nf _ X2). 
+- simpl. destruct S; auto.
+  + simpl. destruct H as [[[[[[[X1 X2] X3] X4] X5] X6] X7] X8]. rewrite X7,X8. apply ltb_asymm. apply ord_lt_ltb. apply ord_succ_not_exp_fp. apply ord_succ_nf. apply ord_max_nf. apply (ptree_ord_nf _ X2). apply (ptree_ord_nf _ X4).
+  + simpl. destruct H as [[[[[[[X1 X2] X3] X4] X5] X6] X7] X8]. rewrite X7,X8. apply ltb_asymm. apply ord_lt_ltb. apply ord_succ_not_exp_fp. apply ord_succ_nf. apply ord_max_nf. apply (ptree_ord_nf _ X2). apply (ptree_ord_nf _ X4).
+  + simpl. destruct H as [[[[[[[X1 X2] X3] X4] X5] X6] X7] X8]. rewrite X7,X8. apply ltb_asymm. apply ord_lt_ltb. apply ord_succ_not_exp_fp. apply ord_succ_nf. apply ord_max_nf. apply (ptree_ord_nf _ X2). apply (ptree_ord_nf _ X4).
+- simpl. destruct S; auto.
+  + simpl. destruct H as [[[[[[[X1 X2] X3] X4] X5] X6] X7] X8]. rewrite X7,X8. apply ltb_asymm. apply ord_lt_ltb. apply ord_succ_not_exp_fp. apply ord_succ_nf. apply ord_max_nf. apply (ptree_ord_nf _ X2). apply (ptree_ord_nf _ X4).
+  + simpl. destruct H as [[[[[[[X1 X2] X3] X4] X5] X6] X7] X8]. rewrite X7,X8. apply ltb_asymm. apply ord_lt_ltb. apply ord_succ_not_exp_fp. apply ord_succ_nf. apply ord_max_nf. apply (ptree_ord_nf _ X2). apply (ptree_ord_nf _ X4).
+  + case (subst_ind_fit f1 S2) eqn:X; auto.
+    * destruct H as [[[[[[[X1 X2] X3] X4] X5] X6] X7] X8]. rewrite X7,X8. destruct S1; simpl.
+      -- admit.
+      -- admit.
+      -- apply ltb_asymm. apply ord_lt_ltb. apply ord_succ_not_exp_fp; apply ord_succ_nf; apply ord_max_nf; try apply (ptree_ord_nf _ X2); apply (ptree_ord_nf _ X4). 
+    * destruct H as [[[[[[[X1 X2] X3] X4] X5] X6] X7] X8]. rewrite X7,X8. apply ltb_asymm. apply ord_lt_ltb. destruct S1; simpl; apply ord_succ_not_exp_fp; apply ord_succ_nf; apply ord_max_nf; try apply (ptree_ord_nf _ X2); apply (ptree_ord_nf _ X4).
+- simpl. destruct S; auto.
+  + simpl. destruct H as [[[X1 X2] X3] X4]. rewrite X4. apply ltb_asymm. apply ord_lt_ltb. apply ord_succ_not_exp_fp. apply ord_succ_nf. apply (ptree_ord_nf _ X2).
+  + simpl. destruct H as [[[X1 X2] X3] X4]. rewrite X4. apply ltb_asymm. apply ord_lt_ltb. apply ord_succ_not_exp_fp. apply ord_succ_nf. apply (ptree_ord_nf _ X2).
+  + simpl. destruct H as [[[X1 X2] X3] X4]. rewrite X4. apply ltb_asymm. apply ord_lt_ltb. apply ord_succ_not_exp_fp. apply ord_succ_nf. apply (ptree_ord_nf _ X2).
+- simpl. destruct S; auto.
+  + simpl. destruct H as [[[X1 X2] X3] X4]. rewrite X4. apply ltb_asymm. apply ord_lt_ltb. apply ord_succ_not_exp_fp. apply ord_succ_nf. apply (ptree_ord_nf _ X2).
+  + simpl. destruct H as [[[X1 X2] X3] X4]. rewrite X4. apply ltb_asymm. apply ord_lt_ltb. apply ord_succ_not_exp_fp. apply ord_succ_nf. apply (ptree_ord_nf _ X2).
+  + case (subst_ind_fit f0 S2) eqn:X; auto.
+    * destruct S1; unfold "&&".
+      --  simpl. destruct H as [[[X1 X2] X3] X4]. rewrite X4. rewrite neg_w_rule_ptree_formula_true. destruct (ord_semiconnex_bool (ord_2_exp (ptree_ord P)) (ptree_ord (neg_w_rule_sub_ptree P Q E F n d' beta HQ (lor_ind (non_target f) S2)))) as [O | [O | O]].
+          ++  apply ltb_asymm. rewrite IHP in O. inversion O. auto.
+          ++  destruct o.
+              ** destruct X4. simpl in O. rewrite (ord_lt_one _ (ord_ltb_lt _ _ O)). auto.
+              ** apply ltb_asymm. apply (ord_ltb_trans _ _ _ (ord_lt_ltb _ _ (ord_lt_succ _ _ (ord_ltb_lt _ _ O)))). apply ord_lt_ltb. apply ord_succ_lt_exp_succ. apply ptree_ord_nf; auto. destruct X4. apply zero_lt.
+          ++  apply ord_eqb_eq in O. destruct O. case (ptree_ord P) eqn:Y; auto. apply ltb_asymm. apply ord_lt_ltb. apply ord_succ_lt_exp_succ. destruct Y. apply ptree_ord_nf; auto. apply zero_lt.
+          ++  rewrite X1. simpl. rewrite non_target_fit. apply X.
+      --  simpl. destruct H as [[[X1 X2] X3] X4]. rewrite X4. rewrite neg_w_rule_ptree_formula_true. destruct (ord_semiconnex_bool (ord_2_exp (ptree_ord P)) (ptree_ord (neg_w_rule_sub_ptree P Q E F n d' beta HQ (lor_ind (non_target f) S2)))) as [O | [O | O]].
+          ++  apply ltb_asymm. rewrite IHP in O. inversion O. auto.
+          ++  destruct o.
+              ** destruct X4. simpl in O. rewrite (ord_lt_one _ (ord_ltb_lt _ _ O)). auto.
+              ** apply ltb_asymm. apply (ord_ltb_trans _ _ _ (ord_lt_ltb _ _ (ord_lt_succ _ _ (ord_ltb_lt _ _ O)))). apply ord_lt_ltb. apply ord_succ_lt_exp_succ. apply ptree_ord_nf; auto. destruct X4. apply zero_lt.
+          ++  apply ord_eqb_eq in O. destruct O. case (ptree_ord P) eqn:Y; auto. apply ltb_asymm. apply ord_lt_ltb. apply ord_succ_lt_exp_succ. destruct Y. apply ptree_ord_nf; auto. apply zero_lt.
+          ++  rewrite X1. simpl. rewrite non_target_fit. apply X.
+      -- destruct H as [[[X1 X2] X3] X4]. rewrite X4. apply ltb_asymm. apply ord_lt_ltb. apply ord_succ_not_exp_fp; apply ord_succ_nf; apply (ptree_ord_nf _ X2). 
+    * destruct H as [[[X1 X2] X3] X4]. rewrite X4. apply ltb_asymm. apply ord_lt_ltb. destruct S1; simpl; apply ord_succ_not_exp_fp; apply ord_succ_nf; apply (ptree_ord_nf _ X2). 
+- admit.
+- admit.
+- simpl. destruct S; auto.
+  + simpl. destruct (H czero) as [[[X1 X2] X3] X4]. rewrite X4. apply ltb_asymm. apply ord_lt_ltb. apply ord_succ_not_exp_fp. apply ord_succ_nf. apply (ptree_ord_nf _ X2).
+  + simpl. destruct (H czero) as [[[X1 X2] X3] X4]. rewrite X4. apply ltb_asymm. apply ord_lt_ltb. apply ord_succ_not_exp_fp. apply ord_succ_nf. apply (ptree_ord_nf _ X2).
+  + simpl. destruct (H czero) as [[[X1 X2] X3] X4]. rewrite X4. apply ltb_asymm. apply ord_lt_ltb. apply ord_succ_not_exp_fp. apply ord_succ_nf. apply (ptree_ord_nf _ X2).
+- simpl. destruct S; auto.
+  + simpl. destruct (H czero) as [[[X1 X2] X3] X4]. rewrite X4. apply ltb_asymm. apply ord_lt_ltb. apply ord_succ_not_exp_fp. apply ord_succ_nf. apply (ptree_ord_nf _ X2).
+  + simpl. destruct (H czero) as [[[X1 X2] X3] X4]. rewrite X4. apply ltb_asymm. apply ord_lt_ltb. apply ord_succ_not_exp_fp. apply ord_succ_nf. apply (ptree_ord_nf _ X2).
+  + case (subst_ind_fit f0 S2); auto.
+    * destruct S1; auto; unfold "&&".
+      --  simpl. destruct (H czero) as [[[X1 X2] X3] X4]. rewrite X4. destruct o.
+          ++  destruct X4. auto.
+          ++  apply ltb_asymm. apply ord_lt_ltb. apply ord_succ_lt_exp_succ. apply ptree_ord_nf; auto. destruct X4. apply zero_lt.
+      --  simpl. destruct (H czero) as [[[X1 X2] X3] X4]. rewrite X4. destruct o.
+          ++  destruct X4. auto.
+          ++  apply ltb_asymm. apply ord_lt_ltb. apply ord_succ_lt_exp_succ. apply ptree_ord_nf; auto. destruct X4. apply zero_lt.
+      -- destruct (H czero) as [[[X1 X2] X3] X4]. rewrite X4. apply ltb_asymm. apply ord_lt_ltb. apply ord_succ_not_exp_fp; apply ord_succ_nf; apply (ptree_ord_nf _ X2).
+    * destruct (H czero) as [[[X1 X2] X3] X4]. rewrite X4. apply ltb_asymm. apply ord_lt_ltb. destruct S1; simpl; apply ord_succ_not_exp_fp; apply ord_succ_nf; apply (ptree_ord_nf _ X2). 
+- simpl. destruct H as [[[[[[[X1 X2] X3] X4] X5] X6] X7] X8]. case (subst_ind_fit f S) eqn:X.
+  + simpl. rewrite neg_w_rule_ptree_formula_true.
+    * case (ord_ltb (ptree_ord (neg_w_rule_sub_ptree P1 Q E F n d' beta HQ (lor_ind S (non_target f0)))) o0) eqn:Y.
+      --  rewrite (ord_max_lem1 _ _ Y). destruct (ord_semiconnex_bool o o0) as [Y1 | [Y1 | Y1]].
+          ++  rewrite ord_max_lem1; auto. apply ltb_asymm. apply ord_lt_ltb. apply ord_succ_not_exp_fp. rewrite X8. apply ord_succ_nf. apply ptree_ord_nf. auto.
+          ++  rewrite ord_max_lem2; auto. apply ltb_asymm. apply ord_lt_ltb. apply (lt_trans _ (ord_2_exp (ord_succ o0))).
+              **  apply ord_succ_not_exp_fp. rewrite X8. apply ord_succ_nf. apply ptree_ord_nf. auto.
+              **  apply ord_2_exp_monot. rewrite X7. apply ord_succ_nf. apply ptree_ord_nf. auto. rewrite X8. apply ord_succ_nf. apply ptree_ord_nf. auto. apply ord_lt_succ. apply ord_ltb_lt. auto.
+              **  apply ltb_asymm. auto.
+          ++  apply ord_eqb_eq in Y1. destruct Y1. rewrite ord_max_lem2; auto. apply ltb_asymm. apply ord_lt_ltb. apply ord_succ_not_exp_fp. rewrite X8. apply ord_succ_nf. apply ptree_ord_nf. auto. apply ord_ltb_irrefl.
+      --  rewrite (ord_max_lem2 _ _ Y). destruct (ord_semiconnex_bool (ord_2_exp (ptree_ord P1)) (ptree_ord (neg_w_rule_sub_ptree P1 Q E F n d' beta HQ (lor_ind S (non_target f0))))) as [Y1 | [Y1 | Y1]].  
+          ++  admit.
+          ++  destruct o.
+              **  destruct X7. simpl in Y1. rewrite (ord_lt_one _ (ord_ltb_lt _ _ Y1)). case (ord_max Zero o0) eqn:Y2; auto. apply ltb_asymm. apply ord_lt_ltb. destruct Y2. apply ord_gt_zero_exp_gt_one.
+                  apply ord_succ_nf. apply ord_max_nf. apply zero_nf. rewrite X8. apply ptree_ord_nf. auto. destruct o0; simpl; auto. apply zero_lt. destruct o0_1; apply zero_lt. 
+              **  apply ltb_asymm. refine (ord_lt_ltb _ _ (lt_trans _ _ _ (ord_lt_succ _ _ (ord_ltb_lt _ _ Y1)) _)). case (ord_ltb (cons o1 n2 o2) o0) eqn:Y2.
+                  { rewrite ord_max_lem1; auto. refine (lt_trans _ _ _ (ord_succ_lt_exp_succ _ _ _) _). apply ptree_ord_nf; auto. destruct X7. apply zero_lt. apply ord_2_exp_monot.
+                    { apply ord_succ_nf. rewrite X8. apply ptree_ord_nf; auto. }
+                    { apply ord_succ_nf. apply ptree_ord_nf; auto. }
+                    { apply ord_lt_succ. destruct X7. apply ord_ltb_lt. auto. } }
+                  { rewrite ord_max_lem2; auto. rewrite X7. apply ord_succ_lt_exp_succ. apply ptree_ord_nf; auto. destruct X7. apply zero_lt. }
+          ++  apply ord_eqb_eq in Y1. destruct Y1. destruct o.
+              **  destruct X7. destruct o0; auto; destruct o0_1; destruct n2; destruct o0_2; inversion Y; auto.          
+              **  rewrite X7. apply ltb_asymm. case (ord_ltb (cons o1 n2 o2) o0) eqn:Y2.
+                  { rewrite ord_max_lem1; auto. apply ord_lt_ltb. refine (lt_trans _ _ _ _ (ord_succ_lt_exp_succ _ _ _)).
+                    { apply ord_lt_succ. apply ord_2_exp_monot.
+                      { rewrite X8. apply ptree_ord_nf; auto. }
+                      { apply ptree_ord_nf; auto. }
+                      { destruct X7. apply ord_ltb_lt. auto. } }
+                    { rewrite X8. apply ptree_ord_nf; auto. }
+                    { destruct o0. inversion Y2. apply zero_lt. }
+                    { destruct X7. auto. } }
+                  { rewrite ord_max_lem2; auto. apply ord_lt_ltb. apply ord_succ_lt_exp_succ. apply ptree_ord_nf; auto. destruct X7. apply zero_lt. destruct X7. auto. }
+    * rewrite X1. simpl. rewrite X. apply non_target_fit.
+  + simpl. rewrite X7,X8. destruct (ord_2_exp_fp _ (ptree_ord_nf _ X2)).
+    * apply ltb_asymm. apply ord_lt_ltb. apply ord_succ_not_exp_fp. apply ord_succ_nf. apply ord_max_nf; apply ptree_ord_nf; auto.
+    * rewrite H. destruct (ord_2_exp_fp _ (ptree_ord_nf _ X4)).
+      -- apply ltb_asymm. apply ord_lt_ltb. apply ord_succ_not_exp_fp. apply ord_succ_nf. apply ord_max_nf; try apply ptree_ord_nf; auto. apply single_nf. apply nf_nat.
+      -- rewrite H0. auto.
+- admit.
+- simpl. destruct S; auto.
+  + simpl. destruct H as [[[[[[[X1 X2] X3] X4] X5] X6] X7] X8]. rewrite X7,X8. apply ltb_asymm. apply ord_lt_ltb. apply ord_succ_not_exp_fp. apply ord_succ_nf. apply ord_max_nf. apply (ptree_ord_nf _ X2). apply (ptree_ord_nf _ X4).
+  + simpl. destruct H as [[[[[[[X1 X2] X3] X4] X5] X6] X7] X8]. rewrite X7,X8. apply ltb_asymm. apply ord_lt_ltb. apply ord_succ_not_exp_fp. apply ord_succ_nf. apply ord_max_nf. apply (ptree_ord_nf _ X2). apply (ptree_ord_nf _ X4).
+  + case (subst_ind_fit f S1 && subst_ind_fit f1 S2); auto.
+    * destruct H as [[[[[[[X1 X2] X3] X4] X5] X6] X7] X8]. rewrite X7,X8.
+      --  simpl. admit.
+    * destruct H as [[[[[[[X1 X2] X3] X4] X5] X6] X7] X8]. rewrite X7,X8. apply ltb_asymm. apply ord_lt_ltb. destruct S1; simpl; apply ord_succ_not_exp_fp; apply ord_succ_nf; apply ord_max_nf; try apply (ptree_ord_nf _ X2); apply (ptree_ord_nf _ X4).
 Admitted.
-
 
 (* Now we prove that if we have a valid ptree, performing our
 w_rule substitution on it results in a valid ptree *)
 (* *)
 Lemma neg_w_rule_valid : forall (P Q : ptree) (E F : formula) (n d' : nat) (beta : ord) (H : P_proves Q (lor F (univ n E)) d' beta),
-  valid P ->
+  valid P -> closed F = true ->
   forall (S : subst_ind),
     subst_ind_fit (ptree_formula P) S = true ->
     valid (neg_w_rule_sub_ptree P Q E F n d' beta H S).
 Proof.
 intros P Q E F n d' beta HQ.
-induction P; try intros H S Hs.
+induction P; try intros H HF S Hs.
 
-- simpl. inversion H as [H1 H2]. inversion Hs. rewrite H3.
-  rewrite neg_w_rule_ptree_formula_true; auto. split.
-  + pose proof (neg_w_rule_ptree_deg P Q E F n d' beta HQ H2 S). lia.
-  + apply (IHP H2 S H3).
+- simpl. inversion H as [H1 H2]. inversion Hs. rewrite H3. case (lt_nat (ptree_deg (neg_w_rule_sub_ptree P Q E F n d' beta HQ S)) n0) eqn:X.
+  + rewrite neg_w_rule_ptree_formula_true; auto. rewrite X. split.
+    * apply lt_nat_decid. auto.
+    * apply (IHP H2 HF S H3).
+  + rewrite neg_w_rule_ptree_formula_true; auto. rewrite X. apply (IHP H2 HF S H3).
 
 - simpl. inversion H as [[H1 H2] H3]. inversion Hs. rewrite H4.
-  rewrite neg_w_rule_ptree_formula_true; auto. split.
-  + rewrite neg_w_rule_ptree_ord; auto.
+  rewrite neg_w_rule_ptree_formula_true; auto. case (ord_ltb (ptree_ord (neg_w_rule_sub_ptree P Q E F n d' beta HQ S)) o) eqn:X.
+  + repeat split; auto. apply ord_ltb_lt. auto.
   + auto.
 
 - simpl. destruct (subst_ind_fit f S); apply H.
 
 - simpl. destruct S; inversion Hs. rewrite H1. simpl.
   inversion H as [[[H2 H3] H4] H5].
-  repeat split; rewrite neg_w_rule_ptree_formula_true.
+  repeat split; rewrite neg_w_rule_ptree_formula_true; auto.
   + rewrite neg_w_rule_ptree_formula; auto.
     rewrite H2. unfold neg_w_rule_sub_formula.
     rewrite formula_sub_ind_lor; auto. apply (and_bool_symm _ _ H1).
   + rewrite H2. simpl. apply (and_bool_symm _ _ H1).
-  + apply IHP. apply H. rewrite H2. simpl. apply (and_bool_symm _ _ H1).
-  + rewrite H2. simpl. apply (and_bool_symm _ _ H1).
-  + rewrite H4. apply (neg_w_rule_ptree_deg P Q E F n d' beta HQ H3 ( lor_ind S2 S1 )).
-  + rewrite H2. simpl. apply (and_bool_symm _ _ H1).
-  + rewrite neg_w_rule_ptree_ord; auto.
+  + apply IHP; auto. rewrite H2. simpl. apply (and_bool_symm _ _ H1).
   + rewrite H2. simpl. apply (and_bool_symm _ _ H1).
 
 - simpl. destruct S; try destruct S1; inversion Hs.
@@ -464,10 +679,6 @@ induction P; try intros H S Hs.
   + rewrite H4. simpl. rewrite H1, H2, H3. auto.
   + apply IHP; auto. rewrite H4. simpl. rewrite H1, H2, H3. auto.
   + rewrite H4. simpl. rewrite H1, H2, H3. auto.
-  + rewrite H6. apply neg_w_rule_ptree_deg; auto.
-  + rewrite H4. simpl. rewrite H1, H2, H3. auto.
-  + rewrite neg_w_rule_ptree_ord; auto.
-  + rewrite H4. simpl. rewrite H1, H2, H3. auto.
 
 - simpl. destruct S; try destruct S1; inversion Hs.
   rewrite H1. simpl. inversion H as [[[H4 H5] H6] H7].
@@ -481,10 +692,6 @@ induction P; try intros H S Hs.
     * simpl. rewrite H1, H2, H3. auto.
   + rewrite H4. simpl. rewrite H1, H2, H3. auto.
   + apply IHP; auto. rewrite H4. simpl. rewrite H1, H2, H3. auto.
-  + rewrite H4. simpl. rewrite H1, H2, H3. auto.
-  + rewrite H6. apply neg_w_rule_ptree_deg; auto.
-  + rewrite H4. simpl. rewrite H1, H2, H3. auto.
-  + rewrite neg_w_rule_ptree_ord; auto.
   + rewrite H4. simpl. rewrite H1, H2, H3. auto.
 
 - simpl. destruct S; try destruct S1; try destruct S1_1; inversion Hs.
@@ -502,10 +709,6 @@ induction P; try intros H S Hs.
   + rewrite H5. simpl. rewrite H0, H2, H3, H4. auto.
   + apply IHP; auto. rewrite H5. simpl. rewrite H0, H2, H3, H4. auto.
   + rewrite H5. simpl. rewrite H0, H2, H3, H4. auto.
-  + rewrite H7. apply neg_w_rule_ptree_deg; auto.
-  + rewrite H5. simpl. rewrite H0, H2, H3, H4. auto.
-  + rewrite neg_w_rule_ptree_ord; auto.
-  + rewrite H5. simpl. rewrite H0, H2, H3, H4. auto.
 
 - simpl. inversion Hs. rewrite H1. inversion H as [[[H2 H3] H4] H5].
   repeat split; rewrite neg_w_rule_ptree_formula_true.
@@ -513,44 +716,30 @@ induction P; try intros H S Hs.
     unfold neg_w_rule_sub_formula. rewrite H2.
     rewrite formula_sub_ind_lor; auto. rewrite H1. auto.
   + rewrite H2. simpl. rewrite H1. auto.
-  + apply IHP. apply H. rewrite H2. simpl. rewrite H1. auto.
-  + rewrite H2. simpl. rewrite H1. auto.
-  + rewrite H4. apply neg_w_rule_ptree_deg; auto.
-  + rewrite H2. simpl. rewrite H1. auto.
-  + rewrite neg_w_rule_ptree_ord; auto.
+  + apply IHP; auto. rewrite H2. simpl. rewrite H1. auto.
   + rewrite H2. simpl. rewrite H1. auto.
 
 - simpl. destruct S; inversion Hs. rewrite H1.
   inversion H as [[[H2 H3] H4] H5]. destruct (and_bool_prop _ _ H1).
   repeat split; rewrite neg_w_rule_ptree_formula_true.
-  + rewrite w_rule_ptree_formula; auto.
+  + rewrite neg_w_rule_ptree_formula; auto.
     unfold neg_w_rule_sub_formula. rewrite H2.
     repeat rewrite formula_sub_ind_lor; auto.
     * rewrite H0. auto.
     * simpl. rewrite H0, H6. auto.
   + rewrite H2. simpl. rewrite H0, H6. auto.
-  + apply IHP. apply H. rewrite H2. simpl. rewrite H0, H6. auto.
-  + rewrite H2. simpl. rewrite H0, H6. auto.
-  + rewrite H4. apply w_rule_ptree_deg; auto.
-  + rewrite H2. simpl. rewrite H0, H6. auto.
-  + rewrite w_rule_ptree_ord; auto.
+  + apply IHP; auto. rewrite H2. simpl. rewrite H0, H6. auto.
   + rewrite H2. simpl. rewrite H0, H6. auto.
 
 - simpl. destruct S; inversion Hs. rewrite H1. simpl.
   inversion H as [[[[H2 H3] H4] H5] H6]. destruct (and_bool_prop _ _ H1).
   repeat split.
-  + rewrite w_rule_ptree_formula_true.
-    * rewrite w_rule_ptree_formula; auto. rewrite H2. auto.
+  + rewrite neg_w_rule_ptree_formula_true.
+    * rewrite neg_w_rule_ptree_formula; auto. rewrite H2. auto.
     * rewrite H2. auto.
-  + apply neg_w_rule_sub_formula_closed. auto.
-  + rewrite w_rule_ptree_formula_true.
+  + apply neg_w_rule_sub_formula_closed; auto.
+  + rewrite neg_w_rule_ptree_formula_true.
     * apply IHP; auto. rewrite H2. auto.
-    * rewrite H2. auto.
-  + rewrite w_rule_ptree_formula_true.
-    * rewrite H5. apply w_rule_ptree_deg; auto.
-    * rewrite H2. auto.
-  + rewrite w_rule_ptree_formula_true.
-    * rewrite w_rule_ptree_ord; auto.
     * rewrite H2. auto.
 
 - simpl. destruct S; apply H.
@@ -558,76 +747,68 @@ induction P; try intros H S Hs.
 - simpl. destruct S; try apply H.
   destruct S1; inversion Hs; rewrite H1; simpl.
   + destruct H as [[[[[[[H2 H3] H4] H5] H6] H7] H8] H9].
-    repeat split; rewrite w_rule_ptree_formula_true.
-    * rewrite w_rule_ptree_formula; auto.
+    repeat split; rewrite neg_w_rule_ptree_formula_true.
+    * rewrite neg_w_rule_ptree_formula; auto.
       rewrite H2. unfold neg_w_rule_sub_formula. rewrite formula_sub_ind_lor.
-      { simpl. destruct (eq_f f (neg E)); auto. }
+      { simpl. destruct (eq_f f (univ n E)); auto. }
       { rewrite H1. auto. }
     * rewrite H2. simpl. apply H1.
     * apply IHP1; auto. rewrite H2. apply H1.
     * rewrite H2. simpl. apply H1.
-    * rewrite w_rule_ptree_formula; auto.
+    * rewrite neg_w_rule_ptree_formula; auto.
       rewrite H4. unfold neg_w_rule_sub_formula. rewrite formula_sub_ind_lor.
-      { simpl. destruct (eq_f f0 (neg E)); auto. }
+      { simpl. destruct (eq_f f0 (univ n E)); auto. }
       { rewrite H1. auto. }
     * rewrite H4. simpl. apply H1.
     * apply IHP2; auto. rewrite H4. simpl. apply H1.
-    * rewrite H4. simpl. apply H1.
-    * rewrite H6. apply w_rule_ptree_deg; auto.
-    * rewrite H2. simpl. apply H1.
-    * rewrite H7. apply w_rule_ptree_deg; auto.
-    * rewrite H4. simpl. apply H1.
-    * rewrite w_rule_ptree_ord; auto.
-    * rewrite H2. simpl. apply H1.
-    * rewrite w_rule_ptree_ord; auto.
     * rewrite H4. simpl. apply H1.
   + destruct H as [[[[[[[H2 H3] H4] H5] H6] H7] H8] H9].
-    repeat split; rewrite w_rule_ptree_formula_true.
-    * rewrite w_rule_ptree_formula; auto.
+    repeat split; rewrite neg_w_rule_ptree_formula_true.
+    * rewrite neg_w_rule_ptree_formula; auto.
       rewrite H2. unfold neg_w_rule_sub_formula. rewrite formula_sub_ind_lor.
-      { simpl. destruct (eq_f f (neg E)); auto. }
+      { simpl. destruct (eq_f f (univ n E)); auto. }
       { rewrite H1. auto. }
     * rewrite H2. simpl. apply H1.
     * apply IHP1; auto. rewrite H2. apply H1.
     * rewrite H2. simpl. apply H1.
-    * rewrite w_rule_ptree_formula; auto.
+    * rewrite neg_w_rule_ptree_formula; auto.
       rewrite H4. unfold neg_w_rule_sub_formula. rewrite formula_sub_ind_lor.
-      { simpl. destruct (eq_f f0 (neg E)); auto. }
+      { simpl. destruct (eq_f f0 (univ n E)); auto. }
       { rewrite H1. auto. }
     * rewrite H4. simpl. apply H1.
     * apply IHP2; auto. rewrite H4. simpl. apply H1.
-    * rewrite H4. simpl. apply H1.
-    * rewrite H6. apply w_rule_ptree_deg; auto.
-    * rewrite H2. simpl. apply H1.
-    * rewrite H7. apply w_rule_ptree_deg; auto.
-    * rewrite H4. simpl. apply H1.
-    * rewrite w_rule_ptree_ord; auto.
-    * rewrite H2. simpl. apply H1.
-    * rewrite w_rule_ptree_ord; auto.
     * rewrite H4. simpl. apply H1.
 
 - simpl. destruct S; destruct (eq_f f E); apply H.
 
 - simpl. inversion H as [[[H1 H2] H3] H4]. destruct S; auto.
   destruct S1; auto; destruct (subst_ind_fit f0 S2) eqn:HS2; simpl;
-  repeat split; auto; rewrite w_rule_ptree_formula_true;
+  repeat split; auto; rewrite neg_w_rule_ptree_formula_true;
   try apply IHP; auto; try rewrite H1; simpl; try rewrite non_target_fit,HS2;
   try rewrite w_rule_ptree_deg; try rewrite w_rule_ptree_ord; auto.
-  + rewrite w_rule_ptree_formula; auto. rewrite H1.
+  + rewrite neg_w_rule_ptree_formula; auto. rewrite H1.
     unfold neg_w_rule_sub_formula. simpl. rewrite non_target_fit,HS2.
     simpl. rewrite <- sub_fit_true; auto.
     * rewrite non_target_sub. rewrite <- sub_fit_true; auto.
     * apply non_target_fit.
-  + rewrite H3. apply w_rule_ptree_deg; auto.
-  + rewrite w_rule_ptree_formula; auto. rewrite H1.
+  + rewrite neg_w_rule_ptree_formula; auto. rewrite H1.
     unfold neg_w_rule_sub_formula. simpl. rewrite non_target_fit,HS2.
     simpl. rewrite <- sub_fit_true; auto.
     * rewrite non_target_sub. rewrite <- sub_fit_true; auto.
     * apply non_target_fit.
-  + rewrite H3. apply w_rule_ptree_deg; auto.
 
-- simpl. destruct S; auto.
+- simpl. destruct S; auto; case (eq_f f E) eqn:X; case (eq_nat n0 n) eqn:X1; auto.
+  apply f_eq_decid in X. destruct X. apply nat_eq_decid in X1. destruct X1.
+  destruct H as [[[X1 X2] X3] X4]. destruct HQ as [[[Y1 Y2 ]Y3] Y4].
+  repeat split; simpl; auto.
+  + rewrite w_rule_ptree_formula; auto. rewrite Y1. unfold w_rule_sub_formula. simpl.
+    rewrite non_target_fit. rewrite eq_nat_refl. rewrite eq_f_refl. simpl. rewrite non_target_sub'. auto. 
+  + apply w_rule_valid; auto. rewrite Y1. simpl. rewrite non_target_fit. auto.
+  + rewrite w_rule_ptree_ord; auto.
 
+- admit.
+
+(*
 - simpl. destruct S; try apply H. inversion H as [[[[H0 H1] H2] H3] H4].
   destruct S1; inversion Hs; rewrite H6; simpl.
   + repeat split; auto.
@@ -662,6 +843,7 @@ induction P; try intros H S Hs.
     * rewrite w_rule_ptree_formula_true.
       { rewrite w_rule_ptree_ord; auto. }
       { rewrite H0. simpl. auto. }
+
 
 - rename f into A. rename p into g. rename n1 into d. rename o into alpha.
   destruct (valid_w_rule_a A n0 d alpha g H m) as [[[H1 H2] H3] H4].
@@ -807,62 +989,75 @@ induction P; try intros H S Hs.
         try rewrite non_target_fit,HS2; auto.
         unfold neg_w_rule_sub_formula. rewrite non_target_sub_lor. auto.
         pose proof (w_rule_ptree_deg (g p) E n m H2 (lor_ind (non_target (substitution A n0 (represent p))) S2 )). lia. }
+*)
+
+- simpl. destruct S; auto.
+
+- simpl. destruct S; try apply H. destruct S1; inversion Hs; rewrite H1; simpl; intros t; destruct (H t) as [[[X1 X2] X3] X4]; fold valid in *.
++ repeat split; auto.
+  * rewrite neg_w_rule_ptree_formula_true, neg_w_rule_ptree_formula; auto.
+    { rewrite X1. unfold neg_w_rule_sub_formula.
+      { rewrite formula_sub_ind_lor.
+        { rewrite (non_target_term_sub _ n0 (projT1 t)). rewrite non_target_sub. auto. }
+        { rewrite (non_target_term_sub _ n0 (projT1 t)). rewrite non_target_fit,H1. auto. } } }
+    { rewrite X1. rewrite (non_target_term_sub _ n0 (projT1 t)). simpl. rewrite non_target_fit,H1. auto. }
+  * rewrite neg_w_rule_ptree_formula_true.
+    { apply X; auto. rewrite X1. rewrite (non_target_term_sub _ n0 (projT1 t)). simpl. rewrite non_target_fit,H1. auto. }
+    { rewrite X1. rewrite (non_target_term_sub _ n0 (projT1 t)). simpl. rewrite non_target_fit,H1. auto. }
+  * admit.
+  * admit.
++ repeat split; auto.
+  * rewrite neg_w_rule_ptree_formula_true, neg_w_rule_ptree_formula; auto.
+    { rewrite X1. unfold neg_w_rule_sub_formula.
+      { rewrite formula_sub_ind_lor. 
+        { rewrite (non_target_term_sub _ n0 (projT1 t)). rewrite non_target_sub. auto. }
+        { rewrite (non_target_term_sub _ n0 (projT1 t)). rewrite non_target_fit,H1. auto. } } }
+    { rewrite X1. rewrite (non_target_term_sub _ n0 (projT1 t)). simpl. rewrite non_target_fit,H1. auto. }
+  * rewrite neg_w_rule_ptree_formula_true.
+    { apply X; auto. rewrite X1. rewrite (non_target_term_sub _ n0 (projT1 t)). simpl. rewrite non_target_fit,H1. auto. }
+    { rewrite X1. rewrite (non_target_term_sub _ n0 (projT1 t)). simpl. rewrite non_target_fit,H1. auto. }
+  * admit.
+  * admit.
 
 - clear IHP2. simpl. destruct (subst_ind_fit f S) eqn:Heq; try apply H. simpl.
   inversion H as [[[[[[[H1 H2] H3] H4] H5] H6] H7] H8].
-  repeat split; auto; rewrite w_rule_ptree_formula_true.
-  + rewrite w_rule_ptree_formula; auto.
+  repeat split; auto; rewrite neg_w_rule_ptree_formula_true.
+  + rewrite neg_w_rule_ptree_formula; auto.
     rewrite H1. unfold neg_w_rule_sub_formula. rewrite formula_sub_ind_lor.
     * rewrite non_target_sub. auto.
     * rewrite Heq, non_target_fit. auto.
   + rewrite H1. simpl. rewrite Heq, non_target_fit. auto.
   + apply IHP1; auto. rewrite H1. simpl. rewrite Heq, non_target_fit. auto.
   + rewrite H1. simpl. rewrite Heq, non_target_fit. auto.
-  + rewrite H5. apply w_rule_ptree_deg; auto.
-  + rewrite H1. simpl. rewrite Heq, non_target_fit. auto.
-  + rewrite w_rule_ptree_ord; auto.
-  + rewrite H1. simpl. rewrite Heq, non_target_fit. auto.
 
 - clear IHP1. simpl. destruct (subst_ind_fit f0 S) eqn:Heq; try apply H. simpl.
   inversion H as [[[[[[[H1 H2] H3] H4] H5] H6] H7] H8].
-  repeat split; auto; rewrite w_rule_ptree_formula_true.
-  + rewrite w_rule_ptree_formula; auto.
+  repeat split; auto; rewrite neg_w_rule_ptree_formula_true.
+  + rewrite neg_w_rule_ptree_formula; auto.
     rewrite H3. unfold neg_w_rule_sub_formula. rewrite formula_sub_ind_lor.
     * rewrite non_target_sub. auto.
     * rewrite Heq, non_target_fit. auto.
   + rewrite H3. simpl. auto.
   + apply IHP2; auto. rewrite H3. simpl. auto.
   + rewrite H3. simpl. auto.
-  + rewrite H6. apply w_rule_ptree_deg; auto.
-  + rewrite H3. simpl. auto.
-  + rewrite w_rule_ptree_ord; auto.
-  + rewrite H3. simpl. auto.
 
 - simpl. inversion H as [[[[[[[H1 H2] H3] H4] H5] H6] H7] H8].
   destruct S; try inversion Hs. rewrite H9.
   destruct (and_bool_prop _ _ H9) as [H10 H11].
-  simpl. repeat split; rewrite w_rule_ptree_formula_true.
-  + rewrite w_rule_ptree_formula; auto.
+  simpl. repeat split; rewrite neg_w_rule_ptree_formula_true.
+  + rewrite neg_w_rule_ptree_formula; auto.
     rewrite H1. unfold neg_w_rule_sub_formula. rewrite formula_sub_ind_lor.
     * rewrite non_target_sub. auto.
     * rewrite H10, non_target_fit. auto.
   + rewrite H1. simpl. rewrite H10, non_target_fit. auto.
   + apply IHP1; auto. rewrite H1. simpl. rewrite H10, non_target_fit. auto.
   + rewrite H1. simpl. rewrite H10, non_target_fit. auto.
-  + rewrite w_rule_ptree_formula; auto.
+  + rewrite neg_w_rule_ptree_formula; auto.
     rewrite H3. unfold neg_w_rule_sub_formula. rewrite formula_sub_ind_lor.
     * rewrite non_target_sub. auto.
     * rewrite H11, non_target_fit. auto.
   + rewrite H3. simpl. auto.
   + apply IHP2; auto. rewrite H3. simpl. auto.
-  + rewrite H3. simpl. auto.
-  + rewrite H5. apply w_rule_ptree_deg; auto.
-  + rewrite H1. simpl. rewrite H10, non_target_fit. auto.
-  + rewrite H6. apply w_rule_ptree_deg; auto.
-  + rewrite H3. simpl. auto.
-  + rewrite w_rule_ptree_ord; auto.
-  + rewrite H1. simpl. rewrite H10, non_target_fit. auto.
-  + rewrite w_rule_ptree_ord; auto.
   + rewrite H3. simpl. auto.
 Qed.
 
